progress in Pipeline: the "explanatory parameters" of the "related"
judgments need to be arguments of "related", not existentials
inside "related", but before composing several "related"s, they have
to be instantiated, so the simulation composition lemma does not notice
them.

Also, a nice code layout BUG (off by one error) is exposed in
PipelineWithRename.v.

compiler/src/compiler/FlatToRiscvSimulation.v
@@ -34,9 +34,17 @@ Section Sim.
        morphism (word.ring_morph (word := Utility.word)),
        constants [word_cst]).
 
-  Definition related: FlatImp.SimState -> MetricRiscvMachine -> Prop :=
+  (* The GhostConsts tell us how to look at the low-level state in order to
+     establish the relationship to the high-level state.
+     Before we can use "related", we will have to provide GhostConsts.
+     In other relations, we might also need to provide more "how to look at"
+     parameters which say things about the interpretation of the high-level
+     and/or low-level state.
+     Since we have to provide GhostConsts from outside, we can also make sure
+     that they match with "how to look at" parameters from the other phases.
+     The argument "pos" is the position of the code relative to program_base. *)
+  Definition related(g: GhostConsts)(pos: Z): FlatImp.SimState -> MetricRiscvMachine -> Prop :=
     fun '(e, c, done, t, m, l) st =>
-      exists (g: GhostConsts) (pos: Z),
         e = g.(e_impl) /\
         fits_stack g.(num_stackwords) g.(e_impl) c /\
         (forall f argnames retnames body,
@@ -61,7 +69,8 @@ Section Sim.
   Axiom TODO_preserve_regs_initialized: forall regs1 regs2,
       regs_initialized regs1 -> regs_initialized regs2.
 
-  Lemma flatToRiscvSim{hyps: @FlatToRiscv.assumptions p}: simulation FlatImp.SimExec FlatToRiscvCommon.runsTo related.
+  Lemma flatToRiscvSim{hyps: @FlatToRiscv.assumptions p}: forall (g: GhostConsts) (pos: Z),
+      simulation FlatImp.SimExec FlatToRiscvCommon.runsTo (related g pos).
   Proof.
     unfold simulation, FlatImp.SimExec, related, FlatImp.SimState.
     intros.
@@ -91,7 +100,6 @@ Section Sim.
     - simpl. intros. simp.
       eexists; split; [|eassumption].
       cbv beta iota.
-      do 2 eexists.
       repeat match goal with
              | |- _ /\ _ => split
              | _ => eapply TODO_preserve_regs_initialized; (eassumption||reflexivity)
